---
jupyter:
  jupytext:
    cell_metadata_filter: -all
    formats: ipynb,md
    main_language: python
    text_representation:
      extension: .md
      format_name: markdown
      format_version: '1.3'
      jupytext_version: 1.18.1
---

<div style="text-align: right;">
written 01/19/2026<br>
<a href="mailto:alex@810lab.com">alex@810lab.com</a>
</div>



# Maxwell's  Operator

## Summary 
We explore  an operator approach to Maxwell's equations, and try to respect differential geometry. 

## Idea 
Consider the following operator :

$$e^{\nabla} = 1+\nabla + \nabla^2 + \ldots$$

Ignore the higher order terms for now. Apply it to the vector potential, $A$.

\begin{align}
e^{\nabla}A &= A+\nabla A + \nabla^2 A = A+F + J
\end{align}

Given the definition of the vector derivative[1], 

$$\nabla \equiv \sum e^i \partial_i .$$
where $e^i \equiv e_i^{-1}$, and $\partial_i \equiv \partial_{e_i}$ is the partial derivative in the $e_i$ direction. This implies 
$$ e^{\nabla} = e^{ \sum e^i \partial_i}  \stackrel{?}{=} \prod e^{ e^i \partial_i}$$

Lets reverse the order of logic and assume $\prod e^{ e^i \partial_i}$ is true. Then under what circumstance does:
$$ \prod e^{ e^i \partial_i}  \stackrel{?}{=} e^{ \sum e^i \partial_i}  $$
expanded in a cartesian frame in STA,
$$ e^{  e^0 \partial_0}e^{  e^1 \partial_1}e^{  e^2 \partial_i}e^{  e^3 \partial_3} 
 \stackrel{?}{=} e^{  e^0 \partial_0 + e^1 \partial_1+  e^2 \partial_i+  e^3 \partial_3}  $$



## Conjugation and Holonomy
The exponential of the partial derivative implements a translation in the independent variable for a *linear* vector manifold.
$$T_{\tau a}f = f(x+\tau a) =  e^{\tau \partial_a}f$$

for a small $\tau$. Since translations commute, 

$$ f(x+\tau a +\epsilon b) = 
e^{\tau \partial_a+\epsilon \partial_{b}}\stackrel{?}{=} 
e^{\tau \partial_a}e^{\epsilon \partial_{b}} $$

Again,  reverse the logic and assume the product of exponentials is true in general, 

$$e^{\tau \partial_a}e^{\epsilon \partial_{b}} \stackrel{?}{=} 
e^{\tau \partial_a+\epsilon \partial_{b}} $$

This is true when $\tau$ and $\epsilon$ are small. But small compared to what? Compared to the curvature. This is  what we are assuming by a *linear* vector manifold. 

Lets consider if we can re-work this in terms of conjugation, because conjugation is  dank. 
 $$ e^{\tau \partial_a}e^{\epsilon \partial_b} fe^{\tilde{\epsilon \partial_b}}e^{\tilde{\tau \partial_a}} 
  =f(x+\tau a +\epsilon b  -\epsilon b -\tau a ) =f(x)  $$
which is a dumb thing to write when we are in a linear space. 

this expresses the fact that a manifold can be approximated as flat for small pertabitations. 
$$\partial_a  \equiv  \frac{f(x)-f(x-\tau a)}{\tau} =
= $$



<!-- #region -->


## Others 
How can split this up by div/curl:

\begin{align}
e^{\nabla}\cdot A &= A + J \\
e^{\nabla}\wedge A &= F
\end{align}


<!-- #endregion -->

## References

[1]  Hestenes, D. (1984). *Clifford Algebra to Geometric Calculus: A Practical Language for Physics*. D. Reidel Publishing Company.




